src/cbor/pulse/raw/CBOR.Pulse.Raw.Nondet.Compare.fst
@@ -1,0 +1,348 @@
+module CBOR.Pulse.Raw.Nondet.Compare
+#lang-pulse
+open CBOR.Pulse.Raw.Match
+open Pulse.Lib.Pervasives
+open CBOR.Pulse.API.Base
+
+module Spec = CBOR.Spec.API.Format
+module Raw = CBOR.Pulse.Raw.Match
+module SpecRaw = CBOR.Spec.Raw
+module Read = CBOR.Pulse.Raw.Read
+module U64 = FStar.UInt64
+module Trade = Pulse.Lib.Trade.Util
+module SZ = FStar.SizeT
+
+inline_for_extraction
+noextract [@@noextract_to "krml"]
+let cbor_nondet_equiv_t =
+  (x1: Raw.cbor_raw) ->
+  (#p1: perm) ->
+  (#v1: Ghost.erased SpecRaw.raw_data_item) ->
+  (x2: Raw.cbor_raw) ->
+  (#p2: perm) ->
+  (#v2: Ghost.erased SpecRaw.raw_data_item) ->
+  stt bool
+  (Raw.cbor_match p1 x1 v1 **
+    Raw.cbor_match p2 x2 v2 **
+    pure (SpecRaw.valid_raw_data_item v1 /\
+      SpecRaw.valid_raw_data_item v2
+    )
+  )
+  (fun res ->
+    Raw.cbor_match p1 x1 v1 **
+    Raw.cbor_match p2 x2 v2 **
+    pure (res == SpecRaw.raw_equiv v1 v2)
+  )
+
+inline_for_extraction
+noextract [@@noextract_to "krml"]
+fn cbor_nondet_setoid_assoc_eq
+  (cbor_nondet_equiv: cbor_nondet_equiv_t)
+  (i1: cbor_map_iterator)
+  (#p1: perm)
+  (#v1: Ghost.erased (list (SpecRaw.raw_data_item & SpecRaw.raw_data_item)))
+  (x2: cbor_map_entry)
+  (#p2: perm)
+  (#v2: Ghost.erased (SpecRaw.raw_data_item & SpecRaw.raw_data_item))
+requires
+  Read.cbor_map_iterator_match p1 i1 v1 **
+  cbor_match_map_entry p2 x2 v2 **
+  pure (
+    List.Tot.for_all SpecRaw.valid_raw_data_item (List.Tot.map fst v1) /\
+    List.Tot.for_all SpecRaw.valid_raw_data_item (List.Tot.map snd v1) /\
+    SpecRaw.valid_raw_data_item (fst v2) /\
+    SpecRaw.valid_raw_data_item (snd v2)
+
+  )
+returns res: bool
+ensures
+  Read.cbor_map_iterator_match p1 i1 v1 **
+  cbor_match_map_entry p2 x2 v2 **
+  pure (res == CBOR.Spec.Util.setoid_assoc_eq SpecRaw.raw_equiv SpecRaw.raw_equiv v1 v2)
+{
+  admit ()
+}
+
+inline_for_extraction
+noextract [@@noextract_to "krml"]
+fn cbor_nondet_list_for_all_setoid_assoc_eq
+  (cbor_nondet_equiv: cbor_nondet_equiv_t)
+  (i1: cbor_map_iterator)
+  (#p1: perm)
+  (#v1: Ghost.erased (list (SpecRaw.raw_data_item & SpecRaw.raw_data_item)))
+  (i2: cbor_map_iterator)
+  (#p2: perm)
+  (#v2: Ghost.erased (list (SpecRaw.raw_data_item & SpecRaw.raw_data_item)))
+requires
+  Read.cbor_map_iterator_match p1 i1 v1 **
+  Read.cbor_map_iterator_match p2 i2 v2 **
+  pure (
+    List.Tot.for_all SpecRaw.valid_raw_data_item (List.Tot.map fst v1) /\
+    List.Tot.for_all SpecRaw.valid_raw_data_item (List.Tot.map snd v1) /\
+    List.Tot.for_all SpecRaw.valid_raw_data_item (List.Tot.map fst v2) /\
+    List.Tot.for_all SpecRaw.valid_raw_data_item (List.Tot.map snd v2)
+  )
+returns res: bool
+ensures
+  Read.cbor_map_iterator_match p1 i1 v1 **
+  Read.cbor_map_iterator_match p2 i2 v2 **
+  pure (res == List.Tot.for_all (CBOR.Spec.Util.setoid_assoc_eq SpecRaw.raw_equiv SpecRaw.raw_equiv v1) v2)
+{
+  admit ()
+}
+
+#push-options "--z3rlimit 32 --print_implicits"
+
+let cbor_array_iterator_match (p: perm) (i: cbor_array_iterator) (l: list SpecRaw.raw_data_item) : slprop =
+  Read.cbor_array_iterator_match p i l
+
+inline_for_extraction noextract [@@noextract_to "krml"]
+let cbor_array_iterator_init :
+  (fits: squash (SZ.fits_u64)) ->
+  (c: cbor_raw) ->
+  (#pm: perm) ->
+  (#r: Ghost.erased SpecRaw.raw_data_item { SpecRaw.Array? r }) ->
+  stt cbor_array_iterator
+(requires
+    (cbor_match pm c r)
+)
+(ensures fun res -> exists* p .
+      cbor_array_iterator_match p res (SpecRaw.Array?.v r) **
+      Trade.trade
+        (cbor_array_iterator_match p res (SpecRaw.Array?.v r))
+        (cbor_match pm c r)
+)
+= Read.cbor_array_iterator_init
+
+inline_for_extraction noextract [@@noextract_to "krml"]
+let cbor_array_iterator_is_empty :
+  (c: cbor_array_iterator) ->
+  (#pm: perm) ->
+  (#r: Ghost.erased (list SpecRaw.raw_data_item)) ->
+stt bool
+(requires
+    cbor_array_iterator_match pm c r
+)
+(ensures fun res ->
+    cbor_array_iterator_match pm c r **
+    pure (res == Nil? r)
+)
+= Read.cbor_array_iterator_is_empty
+
+inline_for_extraction noextract [@@noextract_to "krml"]
+let cbor_array_iterator_next :
+  (sq: squash SZ.fits_u64) ->
+  (pi: ref cbor_array_iterator) ->
+  (#pm: perm) ->
+  (#i: Ghost.erased cbor_array_iterator) ->
+  (#l: Ghost.erased (list SpecRaw.raw_data_item)) ->
+  stt Raw.cbor_raw
+(requires
+    pts_to pi i **
+    cbor_array_iterator_match pm i l **
+    pure (Cons? l)
+)
+(ensures fun res -> exists* a p i' q .
+    cbor_match p res a **
+    pts_to pi i' **
+    cbor_array_iterator_match pm i' q **
+    Trade.trade
+      (cbor_match p res a ** cbor_array_iterator_match pm i' q)
+      (cbor_array_iterator_match pm i l) **
+    pure (Ghost.reveal l == a :: q)
+)
+= Read.cbor_array_iterator_next
+
+inline_for_extraction
+noextract [@@noextract_to "krml"]
+fn cbor_nondet_equiv_body
+  (cbor_nondet_equiv: cbor_nondet_equiv_t)
+: cbor_nondet_equiv_t
+=
+  (x1: _)
+  (#p1: perm)
+  (#v1: Ghost.erased SpecRaw.raw_data_item)
+  (x2: _)
+  (#p2: perm)
+  (#v2: Ghost.erased SpecRaw.raw_data_item)
+{
+  cbor_match_cases x1;
+  cbor_match_cases x2;
+  SpecRaw.valid_eq SpecRaw.basic_data_model v1;
+  SpecRaw.valid_eq SpecRaw.basic_data_model v2;
+  SpecRaw.raw_equiv_eq_valid v1 v2;
+  let mt1 = CBOR.Pulse.Raw.Compare.impl_major_type x1;
+  let mt2 = CBOR.Pulse.Raw.Compare.impl_major_type x2;
+  let _ : squash (SZ.fits_u64) = assume (SZ.fits_u64);
+  if (mt1 <> mt2) {
+    false
+  } else if (mt1 = Spec.cbor_major_type_simple_value) {
+    let w1 = Raw.cbor_match_simple_elim x1;
+    let w2 = Raw.cbor_match_simple_elim x2;
+    (w1 = w2)
+  } else if (mt1 = Spec.cbor_major_type_uint64 || mt1 = Spec.cbor_major_type_neg_int64) {
+    let w1 = Raw.cbor_match_int_elim_value x1;
+    let w2 = Raw.cbor_match_int_elim_value x2;
+    ((w1.value <: U64.t) = w2.value)
+  } else if (mt1 = Spec.cbor_major_type_byte_string || mt1 = Spec.cbor_major_type_text_string) {
+    let len1 = Raw.cbor_match_string_elim_length x1;
+    let len2 = Raw.cbor_match_string_elim_length x2;
+    if ((len1.value <: U64.t) <> len2.value) {
+      false
+    } else {
+      let w1 = Raw.cbor_match_string_elim_payload x1;
+      let w2 = Raw.cbor_match_string_elim_payload x2;
+      let res = CBOR.Pulse.Raw.Compare.Bytes.lex_compare_bytes w1 w2;
+      CBOR.Spec.Raw.Format.bytes_lex_compare_equal (SpecRaw.String?.v v1) (SpecRaw.String?.v v2);
+      Trade.elim _ (cbor_match p1 x1 v1);
+      Trade.elim _ _;
+      (res = 0s)
+    }
+  } else if (mt1 = Spec.cbor_major_type_tagged) {
+    if (Raw.CBOR_Case_Serialized_Tagged? x1 && Raw.CBOR_Case_Serialized_Tagged? x2) {
+      norewrite let Raw.CBOR_Case_Serialized_Tagged cs1 = x1;
+      norewrite let Raw.CBOR_Case_Serialized_Tagged cs2 = x2;
+      Trade.rewrite_with_trade
+        (cbor_match p1 x1 v1)
+        (cbor_match_serialized_tagged cs1 p1 v1);
+      Trade.rewrite_with_trade
+        (cbor_match p2 x2 v2)
+        (cbor_match_serialized_tagged cs2 p2 v2);
+      let res = CBOR.Pulse.Raw.Format.Nondet.Compare.cbor_match_equal_serialized_tagged cs1 cs2;
+      Trade.elim _ (cbor_match p1 x1 v1);
+      Trade.elim _ _;
+      res
+    } else {
+      let tag1 = Raw.cbor_match_tagged_get_tag x1;
+      let tag2 = Raw.cbor_match_tagged_get_tag x2;
+      if ((tag1.value <: U64.t) <> tag2.value) {
+        false
+      } else {
+        let w1 = Read.cbor_match_tagged_get_payload x1;
+        let w2 = Read.cbor_match_tagged_get_payload x2;
+        let res = cbor_nondet_equiv w1 w2;
+        Trade.elim _ (cbor_match p1 x1 v1);
+        Trade.elim _ _;
+        res
+      }
+    }
+  } else if (mt1 = Spec.cbor_major_type_array) {
+    if (Raw.CBOR_Case_Serialized_Array? x1 && Raw.CBOR_Case_Serialized_Array? x2) {
+      norewrite let Raw.CBOR_Case_Serialized_Array cs1 = x1;
+      norewrite let Raw.CBOR_Case_Serialized_Array cs2 = x2;
+      Trade.rewrite_with_trade
+        (cbor_match p1 x1 v1)
+        (cbor_match_serialized_array cs1 p1 v1);
+      Trade.rewrite_with_trade
+        (cbor_match p2 x2 v2)
+        (cbor_match_serialized_array cs2 p2 v2);
+      let res = CBOR.Pulse.Raw.Format.Nondet.Compare.cbor_match_compare_serialized_array cs1 cs2;
+      Trade.elim _ (cbor_match p1 x1 v1);
+      Trade.elim _ _;
+      res
+    } else {
+      let len1 = Raw.cbor_match_array_get_length x1;
+      let len2 = Raw.cbor_match_array_get_length x2;
+      Classical.move_requires (CBOR.Spec.Util.list_for_all2_length SpecRaw.raw_equiv (SpecRaw.Array?.v v1)) (SpecRaw.Array?.v v2);
+      if ((len1.value <: U64.t) <> len2.value) {
+        false
+      } else {
+        let i1 = cbor_array_iterator_init () x1;
+        let i2 = cbor_array_iterator_init () x2;
+        let mut pi1 = i1;
+        let mut pi2 = i2;
+        let mut pres = true;
+        while (
+          if (!pres) {
+            let i1 = !pi1;
+            not (cbor_array_iterator_is_empty i1)
+          } else {
+            false
+          }
+        ) invariant b . exists* i1 i2 res l1 l2 pj1 pj2 . (
+          pts_to pi1 i1 **
+          pts_to pi2 i2 **
+          pts_to pres res **
+          cbor_array_iterator_match pj1 i1 l1 **
+          cbor_array_iterator_match pj2 i2 l2 **
+          Trade.trade
+            (cbor_array_iterator_match pj1 i1 l1)
+            (cbor_match p1 x1 v1) **
+          Trade.trade
+            (cbor_array_iterator_match pj2 i2 l2)
+            (cbor_match p2 x2 v2) **
+          pure (
+            List.Tot.length l1 == List.Tot.length l2 /\
+            List.Tot.for_all SpecRaw.valid_raw_data_item l1 /\
+            List.Tot.for_all SpecRaw.valid_raw_data_item l2 /\
+            b == (Cons? l1 && res) /\
+            (SpecRaw.raw_equiv v1 v2 == (res && CBOR.Spec.Util.list_for_all2 SpecRaw.raw_equiv l1 l2))
+        )) {
+          let y1 = cbor_array_iterator_next () pi1;
+          Trade.trans _ _ (cbor_match p1 x1 v1);
+          let y2 = cbor_array_iterator_next () pi2;
+          Trade.trans _ _ (cbor_match p2 x2 v2);
+          pres := cbor_nondet_equiv y1 y2;
+          Trade.elim_hyp_l _ _ (cbor_match p1 x1 v1);
+          Trade.elim_hyp_l _ _ (cbor_match p2 x2 v2);
+        };
+        Trade.elim _ (cbor_match p1 x1 v1);
+        Trade.elim _ _;
+        !pres
+      }
+    }
+  } else {
+    assert (pure (mt1 == Spec.cbor_major_type_map));
+    if (Raw.CBOR_Case_Serialized_Map? x1 && Raw.CBOR_Case_Serialized_Map? x2) {
+      norewrite let Raw.CBOR_Case_Serialized_Map cs1 = x1;
+      norewrite let Raw.CBOR_Case_Serialized_Map cs2 = x2;
+      Trade.rewrite_with_trade
+        (cbor_match p1 x1 v1)
+        (cbor_match_serialized_map cs1 p1 v1);
+      Trade.rewrite_with_trade
+        (cbor_match p2 x2 v2)
+        (cbor_match_serialized_map cs2 p2 v2);
+      let res = CBOR.Pulse.Raw.Format.Nondet.Compare.cbor_match_compare_serialized_map cs1 cs2;
+      Trade.elim _ (cbor_match p1 x1 v1);
+      Trade.elim _ _;
+      res
+    } else {
+      let i1 = Read.cbor_map_iterator_init () x1;
+      let i2 = Read.cbor_map_iterator_init () x2;
+      if (not (cbor_nondet_list_for_all_setoid_assoc_eq cbor_nondet_equiv i2 i1)) {
+        Trade.elim _ (cbor_match p1 x1 v1);
+        Trade.elim _ _;
+        false
+      } else {
+        let res = cbor_nondet_list_for_all_setoid_assoc_eq cbor_nondet_equiv i1 i2;
+        Trade.elim _ (cbor_match p1 x1 v1);
+        Trade.elim _ _;
+        res
+      }
+    }
+  }
+}
+
+#pop-options
+
+fn rec cbor_nondet_equiv
+  (x1: _)
+  (#p1: perm)
+  (#v1: Ghost.erased SpecRaw.raw_data_item)
+  (x2: _)
+  (#p2: perm)
+  (#v2: Ghost.erased SpecRaw.raw_data_item)
+requires
+  Raw.cbor_match p1 x1 v1 **
+  Raw.cbor_match p2 x2 v2 **
+  pure (SpecRaw.valid_raw_data_item v1 /\
+    SpecRaw.valid_raw_data_item v2
+  )
+returns res: bool
+ensures
+  Raw.cbor_match p1 x1 v1 **
+  Raw.cbor_match p2 x2 v2 **
+  pure (res == SpecRaw.raw_equiv v1 v2)
+{
+  cbor_nondet_equiv_body cbor_nondet_equiv x1 x2
+}
